Updated Browser.fst - it now compiles
Small changes for nfact authentication in the protocol

Code/AuthenticationProvider.fst
@@ -16,6 +16,20 @@ let createAssertion me user idp =
 	EncryptAssertion idp pubkidp signAssertion
 *)
 
+val nfactauth: me:prin -> idp:prin -> name:string -> assertion:Assertion -> unit
+
+let nfactauth me idp name assertion =
+	if (allnfactauthed name) then
+		resetnfact name;
+		let status = "OK" in
+		let resp = LoginSuccess status me idp assertion in
+		SendSaml idp resp
+	else
+		let challenge = GenerateNonce me in
+		let authmethod = getnfactor name in
+		let resp = LoginResponseMessage me idp assertion authmethod challenge in
+		SendSaml idp resp
+
 val authenticationprovider: me:prin -> idp:prin -> user:prin -> unit
 
 let rec authenticationprovider me idp user =
@@ -27,7 +41,7 @@ let rec authenticationprovider me idp user =
 			(assert (Log issuer message);
 			match loginInfo with
 			| UserLogin(name, password) ->
-				if (revokedidp name idp) && (checklogin name password) then
+				if not (revokedidp name idp) && (checklogin name password) then
 					(*Find the n-factor auth method - How / which one if more?*)
 					let challenge = GenerateNonce me in
 					let assertion = MakeAssertion me user idp in
@@ -50,15 +64,14 @@ let rec authenticationprovider me idp user =
 		else
 			SendSaml idp (Failed Requester);
 			authenticationprovider me idp user
-	| SecondAuthRequest(issuer, destination, message, authInfo, challenge, sigIdP)->
+	| NfactAuthRequest(issuer, destination, message, authInfo, challenge, sigIdP)->
 		(*Associate the challenge to the challenge generated at the first login*)
 		let pubkissuer = CertStore.GetPublicKey issuer in
 		if (whitelisted idp) && (VerifySignature issuer pubkissuer message sigIdP) then
 			(assert (Log issuer message);
 			match authInfo with
 			| UserAuth(name, auth) ->
-				if (revokedidp name idp) && (checknfactor name auth) then
-					let status = "OK" in
+				if not (revokedidp name idp) && (checknfactor name auth) then
 					let assertion = MakeAssertion me user idp in
 					let myprivk = CertStore.GetPrivateKey me in
 					assume(Log me assertion);
@@ -66,8 +79,7 @@ let rec authenticationprovider me idp user =
 					let sigAs = Sign me myprivk assertion in
 					let signAssertion = AddSignatureToAssertion assertion sigAs in
 					let assertion = EncryptAssertion idp pubkidp signAssertion in
-					let resp = LoginSuccess status me idp assertion in
-					SendSaml idp resp;
+					nfactauth me name idp assertion;
 					authenticationprovider me idp user
 				else
 					SendSaml idp (Failed User);
