Code/Browser.fst
@@ -1,11 +1,59 @@
 module Browser
 
 open SamlProtocol
+open Crypto
 
+val loginWithFb: Authentication
+val loginWithGoogle: Authentication
+val loginWithSMS: Authentication
+val loginWithOpenId: Authentication
+val fakeprint: str:string -> unit
 (*Handle the two-factor authentication*)
-val browser: sp:prin -> idp:prin -> res:uri -> user:string -> password:string -> unit
 
-let browser idp resource user password =
-	let req = SPLogin "Login" in
+val handleAuthMethod: auth:Authentication -> Authentication
+
+let handleAuthMethod auth = 
+	match auth with
+	| Facebook(fbid) -> loginWithFb
+	| Google(gid) -> loginWithGoogle
+	| SMS(gen) -> loginWithSMS
+	| OpenId(oid) -> loginWithOpenId
+					
+val loop: user:string -> idp:prin -> sp:prin -> unit
+
+let rec loop user idp sp =
+	let loginresp = ReceiveSaml idp in
+		match loginresp with
+		| UserAuthRequest(authmethod, challenge) ->
+			let authtry = handleAuthMethod authmethod in
+			let authInfo = UserAuth user authtry in
+			let authresp = UserAuthResponse authInfo challenge in
+			SendSaml idp authresp;
+			loop user idp sp
+		| AuthResponseMessage(idenp, dest, assertion) ->
+			SendSaml sp loginresp
+		| _ -> loginresp; ()
+
+val browser: sp:prin -> res:uri -> user:string -> password:string -> unit
+
+let browser sp resource user password =
+	let req = SPLogin resource in
 	let _ = SendSaml sp req in
 		let res = ReceiveSaml sp in
+		match res with
+		| AuthnRequestMessage(sp, idp, message, sigSP) ->
+			SendSaml idp res;
+			let idpResp = ReceiveSaml idp in
+			match idpResp with
+			| UserCredRequest(challenge) ->
+				let loginInfo = UserLogin user password in
+				let loginreq = Login loginInfo challenge in
+				SendSaml idp loginreq;
+				loop user idp sp;
+				let spResp = ReceiveSaml sp in
+					match spResp with
+					| LoginResponse(str) ->
+							fakeprint str
+					| _ -> spResp; ()
+			| _ -> idpResp; ()
+		| _ -> res; ()
